TP Compilation

Tactics.v
@@ -1,71 +1,44 @@
+Require Import Bool.
+
+Definition proj_sumbool {X Y} (x: {X} + {Y}) := if x then true else false.
+
+Coercion proj_sumbool: sumbool >-> bool.
+
+Lemma proj_sumbool_rewrites:
+  forall {E} x y (a b: E),
+  (if x && y then a else b) =
+  if x then if y then a else b else b.
+Proof.
+  intros.
+  destruct x, y; simpl in *; try congruence.
+Qed.
+
+
 Ltac inv H := inversion H; try subst; clear H.
 
+Ltac destr_term t :=
+  match t with
+  | context [if ?a then _ else _] => destruct a eqn:?
+  | context [match ?a with _ => _ end] => destruct a eqn:?
+  | _ => destruct t eqn:?
+  end.
+
+Ltac destr :=
+  match goal with
+  | |- context [if ?a then _ else _] => destr_term a
+  | |- context [match ?a with _ => _ end] => destr_term a
+  end.
+
+Ltac destr_in H :=
+  match type of H with
+  | context [if ?a then _ else _] => destr_term a
+  | context [match ?a with _ => _ end] => destr_term a
+  end.
 
 Ltac trim H :=
   match type of H with
-    ?A -> ?B => let x := fresh in
-                assert (x: A); [clear H| specialize (H x); clear x]
+  | ?a -> ?b =>
+    let x := fresh in
+    assert (x: a); [|specialize (H x); clear x]
   end.
-
-Require Import Arith ZArith Lia.
-
-Definition Zfact n := Z.of_nat (fact (Z.to_nat n)).
-
-Lemma fact_S:
-  (forall n : nat,
-    n <> 0 ->
-    fact n = n * fact (n - 1))%nat.
-Proof.
-  destruct n; simpl; auto. congruence.
-  rewrite ! Nat.sub_0_r.  auto.
-Qed.
-
-Open Scope Z_scope.
-
-Lemma Zfact_pos:
-  forall z, 0 < z ->
-            Zfact z = z * Zfact (z - 1).
-Proof.
-  unfold Zfact. intros.
-  rewrite (fact_S (Z.to_nat z)). 2: lia.
-  rewrite Z2Nat.inj_sub. simpl. 2: lia.
-  rewrite Nat2Z.inj_mul.
-  rewrite Z2Nat.id. 2: lia. reflexivity.
-Qed.
-
-Lemma Zfact_neg:
-  forall z,
-    z <= 0 ->
-    Zfact z = 1.
-Proof.
-  unfold Zfact; intros.
-  unfold Z.to_nat.
-  destruct z; simpl; auto. lia.
-Qed.
-
-
-Fixpoint fib n :=
-  (match n with
-  | O => 1%nat
-  | S n' => match n' with
-            | O => 1
-            | S n'' => fib n' + fib n''
-            end
-  end)%nat.
-
-Lemma fib_eqn (n: nat) : (n > 0 -> fib n + fib (Nat.pred n) = fib (1 + n))%nat.
-Proof.
-  induction n; simpl; intros; eauto. lia.
-Qed.
-
-Definition Zfib n := Z.of_nat (fib (Z.to_nat n)).
-
-Lemma Zfib_eqn (n: Z) : n > 0 -> Zfib n + Zfib (n - 1) = Zfib (1 + n).
-Proof.
-  unfold Zfib. intros.
-  rewrite Z2Nat.inj_add by lia.
-  rewrite Z2Nat.inj_sub by lia.
-  rewrite <- fib_eqn by lia. f_equal.
-  rewrite <- Nat2Z.inj_add. f_equal. f_equal. f_equal. lia.
-Qed.
 
