Fac.v
@@ -1,0 +1,17 @@
+Require Import While String.
+Require Import ZArith.
+Open Scope Z_scope.
+
+Definition fac :=
+  Seq
+    (Assign "res" (Const 1))
+    (Seq
+       (While (Lt (Const 0) (Var "n"))
+              (Seq
+                 (Assign "res" (Binop Bmul (Var "res") (Var "n")))
+                 (Assign "n" (Binop Bsub (Var "n") (Const 1)))
+              )
+       )
+       (Output (Var "res"))
+    ).
+
